mark-and-sweep/spec/GC.Spec.Allocator.Lemmas.SearchChain.fsti
@@ -10,7 +10,7 @@ module Seq = FStar.Seq
 
 val alloc_spec_preserves_fl_chain_terminates : (g: heap) -> (fp: U64.t) -> (requested_wz: nat) ->
   Lemma (requires well_formed_heap g /\
-                  GC.Spec.Allocator.Lemmas.Common.fl_valid g fp (heap_size / U64.v mword) /\
-                  GC.Spec.Allocator.Lemmas.Chain.fl_chain_terminates g fp (heap_size / U64.v mword))
+                  GC.Spec.Allocator.Lemmas.Common.fl_valid g fp alloc_search_fuel /\
+                  GC.Spec.Allocator.Lemmas.Chain.fl_chain_terminates g fp alloc_search_fuel)
         (ensures (let r = alloc_spec g fp requested_wz in
-                  GC.Spec.Allocator.Lemmas.Chain.fl_chain_terminates r.heap_out r.fp_out (heap_size / U64.v mword)))
+                  GC.Spec.Allocator.Lemmas.Chain.fl_chain_terminates r.heap_out r.fp_out alloc_search_fuel))
